nrjgwrgöj

Games/gameLib_fix/Zermelo_brandNew.lean
@@ -33,18 +33,118 @@ lemma Hist_legal_rtake_fst (ini : α) (f_law s_law : α → List β → (β → 
   rw [if_pos htT] at now
   exact now
 
+lemma Hist_legal_rtake_snd (ini : α) (f_law s_law : α → List β → (β → Prop)) (hist : List β) (t : Nat) (htT : Turn_snd (t+1)) (htL : t < hist.length)
+  (main : Hist_legal ini f_law s_law hist) : s_law ini (hist.rtake t) (hist.rget ⟨t, htL⟩) := by
+  replace main := Hist_legal_rtake _ _ _ _ (t+1) main
+  rw [@List.rget_cons_rtake _ _ ⟨t,htL⟩ ] at main
+  cases' main
+  rename_i _ now
+  rw [List.length_rtake (le_of_lt htL)] at now
+  rw [Turn_snd_iff_not_fst] at htT
+  rw [if_neg htT] at now
+  exact now
+
+
+
+def fStrat_staged (ini : α) (f_law s_law : α → List β → (β → Prop)) (f_strat : fStrategy ini f_law s_law) (hist : List β) (leg : Hist_legal ini f_law s_law hist) : Prop :=
+ ∀ t, (ht : t < hist.length) → (T : Turn_fst (t+1)) →  f_strat (hist.rtake t) (by rw [List.length_rtake (le_of_lt ht)] ; exact T) (Hist_legal_rtake _ _ _ _ _ leg) = ⟨ hist.rget ⟨t,ht⟩ , (Hist_legal_rtake_fst _ _ _ _ _ T ht leg)⟩
+
+
+def fStrat_wHist (ini : α) (f_law s_law : α → List β → (β → Prop)) (hist : List β) (leg : Hist_legal ini f_law s_law hist) :=
+  { f_strat : fStrategy ini f_law s_law // fStrat_staged ini f_law s_law f_strat hist leg}
+
+
+def sStrat_staged (ini : α) (f_law s_law : α → List β → (β → Prop)) (s_strat : sStrategy ini f_law s_law) (hist : List β) (leg : Hist_legal ini f_law s_law hist) : Prop :=
+ ∀ t, (ht : t < hist.length) → (T : Turn_snd (t+1)) →  s_strat (hist.rtake t) (by rw [List.length_rtake (le_of_lt ht)] ; exact T) (Hist_legal_rtake _ _ _ _ _ leg) = ⟨ hist.rget ⟨t,ht⟩ , (Hist_legal_rtake_snd _ _ _ _ _ T ht leg)⟩
+
+
+def sStrat_wHist (ini : α) (f_law s_law : α → List β → (β → Prop)) (hist : List β) (leg : Hist_legal ini f_law s_law hist) :=
+  { s_strat : sStrategy ini f_law s_law // sStrat_staged ini f_law s_law s_strat hist leg}
+
+
+def Game_World.is_fst_staged_win  {α β : Type _} (g : Game_World α β) (hist : List β) (leg : Hist_legal g.init_game_state g.fst_legal g.snd_legal hist) : Prop :=
+  ∃ ws : fStrat_wHist g.init_game_state g.fst_legal g.snd_legal hist leg,
+  ∀ snd_s : sStrat_wHist g.init_game_state g.fst_legal g.snd_legal hist leg,
+  ({g with fst_strat := ws.val, snd_strat := snd_s.val} : Game α β).fst_win
+
+def Game_World.is_snd_staged_win  {α β : Type _} (g : Game_World α β) (hist : List β) (leg : Hist_legal g.init_game_state g.fst_legal g.snd_legal hist) : Prop :=
+  ∃ ws : sStrat_wHist g.init_game_state g.fst_legal g.snd_legal hist leg,
+  ∀ fst_s : fStrat_wHist g.init_game_state g.fst_legal g.snd_legal hist leg,
+  ({g with fst_strat := fst_s.val, snd_strat := ws.val} : Game α β).snd_win
+
+
+inductive Game_World.has_staged_WL (g : Game_World α β) (hist : List β) (leg : Hist_legal g.init_game_state g.fst_legal g.snd_legal hist) : Prop where
+| wf (h : g.is_fst_staged_win hist leg)
+| ws (h : g.is_snd_staged_win hist leg)
+
+lemma fStrat_staged_empty (ini : α) (f_law s_law : α → List β → (β → Prop)) (f_strat : fStrategy ini f_law s_law) :
+  fStrat_staged ini f_law s_law f_strat [] Hist_legal.nil := by
+  intro _ no
+  contradiction
+
+lemma sStrat_staged_empty (ini : α) (f_law s_law : α → List β → (β → Prop)) (s_strat : sStrategy ini f_law s_law) :
+  sStrat_staged ini f_law s_law s_strat [] Hist_legal.nil := by
+  intro _ no
+  contradiction
+
+lemma Game_World.has_WL_iff_has_staged_WL_empty (g : Game_World α β) :
+  g.has_WL ↔ g.has_staged_WL [] Hist_legal.nil :=
+  by
+  constructor
+  · intro h
+    cases' h with h h
+    · obtain ⟨ws, ws_prop⟩ := h
+      apply Game_World.has_staged_WL.wf
+      use ⟨ws, fStrat_staged_empty g.init_game_state g.fst_legal g.snd_legal ws⟩
+      intro s_strat
+      exact ws_prop s_strat.val
+    · obtain ⟨ws, ws_prop⟩ := h
+      apply Game_World.has_staged_WL.ws
+      use ⟨ws, sStrat_staged_empty g.init_game_state g.fst_legal g.snd_legal ws⟩
+      intro s_strat
+      exact ws_prop s_strat.val
+  · intro h
+    cases' h with h h
+    · obtain ⟨ws, ws_prop⟩ := h
+      apply Game_World.has_WL.wf
+      use ws.val
+      intro s_strat
+      exact ws_prop ⟨s_strat, sStrat_staged_empty g.init_game_state g.fst_legal g.snd_legal s_strat⟩
+    · obtain ⟨ws, ws_prop⟩ := h
+      apply Game_World.has_WL.ws
+      use ws.val
+      intro s_strat
+      exact ws_prop ⟨s_strat, fStrat_staged_empty g.init_game_state g.fst_legal g.snd_legal s_strat⟩
+
+
+lemma Game_World.has_WL_helper (g : Game_World α β) (hist : List β) (leg : Hist_legal g.init_game_state g.fst_legal g.snd_legal hist) :
+  g.has_staged_WL hist leg → (¬ g.is_fst_staged_win hist leg) → g.is_snd_staged_win hist leg := by
+  intro m c
+  cases' m with m m
+  · exfalso ; exact c m
+  · exact m
+
+lemma Game_World.conditioning_step (g : Game_World α β) (t : Nat)
+  (main : ∀ hist : List β, (leg : Hist_legal g.init_game_state g.fst_legal g.snd_legal hist) → hist.length = t+1 → g.has_staged_WL hist leg) :
+  ∀ hist : List β, (leg : Hist_legal g.init_game_state g.fst_legal g.snd_legal hist) → hist.length = t → g.has_staged_WL hist leg := by
+  intro hist leg len
+  by_cases T : Turn_fst (t+1)
+  · by_cases q : ∃ f_act : β, ∃ (al : g.fst_legal g.init_game_state hist f_act), (g.is_fst_staged_win (f_act :: hist) (Hist_legal.cons hist f_act (by rw [len, if_pos T] ; exact al) leg))
+    · sorry
+    · push_neg at q
+      have main' : ∀ (f_act : β) (al : fst_legal g g.init_game_state hist f_act), g.is_snd_staged_win (f_act :: hist) (Hist_legal.cons hist f_act (by rw [len, if_pos T] ; exact al) leg) :=
+        by
+        intro f_act al
+        specialize main (f_act :: hist) (Hist_legal.cons hist f_act (by rw [len, if_pos T] ; exact al) leg) (by rw [List.length_cons, len])
+        specialize q f_act al
+        exact g.has_WL_helper (f_act :: hist) (Hist_legal.cons hist f_act (by rw [len, if_pos T] ; exact al) leg) main q
+      sorry
+  · sorry
+
+
 
 
 #exit
-
-def fStrat_staged (ini : α) (f_law s_law : α → List β → (β → Prop)) (f_strat : fStrategy ini f_law s_law) (hist : List β) : Prop :=
- ∀ t, (ht : t < hist.length) → (T : Turn_fst (t+1)) → f_strat (hist.rtake t) (by rw [List.length_rtake (le_of_lt ht)] ; exact T) sorry = ⟨ hist.get ⟨t,ht⟩ , sorry⟩
-
-
-
-def fStrat_wHist (ini : α) (f_law s_law : α → List β → (β → Prop)) (hist : List β) :=
-  { f_strat : fStrategy ini f_law s_law // fStrat_staged ini f_law s_law f_strat hist}
-
 
 -- # Zermelo
 
