Games/gameLib_fix/Termination.lean
@@ -103,9 +103,9 @@ def Game_World.is_fst_win  {α β : Type _} (g : Game_World α β) : Prop :=
   ({g with fst_strat := ws, snd_strat := snd_s} : Game α β).fst_win
 
 def Game_World.is_snd_win  {α β : Type _} (g : Game_World α β) : Prop :=
-  ∃ ws : fStrategy g.init_game_state g.fst_legal g.snd_legal,
-  ∀ snd_s : sStrategy g.init_game_state g.fst_legal g.snd_legal,
-  ({g with fst_strat := ws, snd_strat := snd_s} : Game α β).snd_win
+  ∃ ws : sStrategy g.init_game_state g.fst_legal g.snd_legal,
+  ∀ fst_s : fStrategy g.init_game_state g.fst_legal g.snd_legal,
+  ({g with fst_strat := fst_s, snd_strat := ws} : Game α β).snd_win
 
 def Symm_Game_World.is_fst_win  {α β : Type _} (g : Symm_Game_World α β) : Prop :=
   g.toGame_World.is_fst_win
